Progress

LTS.v
@@ -64,7 +64,8 @@ Section ETL.
     }.
 
   (* Each agent has a program -- a binary relation on (heap * prog) *)
-  Variable (transition: uid -> relation (heap*prog)).
+  Variable (transition: uid -> heap*prog -> heap*prog -> Prop).
+  Variable (transition_trans: forall u, transitive _ (transition u)).
   
   (* Transition function is functional & deterministic *)
   Variable (transition_determ: forall u s s' s'',
@@ -112,6 +113,12 @@ Section ETL.
   (* Transitive-reflexive closure of step *)
   Notation "a '==>*' b" := (step ^* a b) (at level 40).
 
+  (**************** Run the system ***************)
+  Inductive Run: system -> Prop :=
+    DoRun: forall s s', init_system s ->
+           s ==>* s' ->
+           Run s'.
+  
   (***************** Logic ********************)
   Definition systemProp := (system -> Prop).
   Definition traceProp := (trace -> Prop).
@@ -119,10 +126,16 @@ Section ETL.
   Definition atomProp := (atom -> Prop).
   Definition factProp := (fact -> Prop).
 
-  (***************** Focusing different parts of the logic ******************)
-  Definition system2trace(P: systemProp): traceProp :=
-    fun str => P ([str]).
+  (***************** Lifting ******************)
+  Definition reflect(P: systemProp): Prop :=
+    forall s, Run s -> P s.
+  
+  Definition trace2system(P: traceProp): systemProp :=
+    fun s => List.Forall P s.
 
+  Definition system2trace(P: systemProp): traceProp :=
+    fun str => P [str].
+  
   Definition state2trace(P: stateProp): traceProp :=
     fun str => P (hd str).
 
@@ -131,49 +144,63 @@ Section ETL.
 
   Inductive atom2fact(P: atomProp): factProp :=
     RetValid: forall a, P a -> atom2fact P (Ret a).
+
+  Arguments reflect /.
+  Coercion system2trace: systemProp >-> traceProp.
+  Coercion trace2system: traceProp >-> systemProp.
+  Coercion state2trace: stateProp >-> traceProp.
+  Coercion fact2state: factProp >-> stateProp.
+  Coercion atom2fact: atomProp >-> factProp.
+
+  (***************** Intuitionistic logic  *******************)
+  Global Instance ILogicOps_systemProp : ILogicOps systemProp := _.
+  Global Instance ILogicOps_traceProp : ILogicOps traceProp := _.
+  Global Instance ILogicOps_stateProp : ILogicOps stateProp := _.
   
   (********************** Path restriction *******************)
   Definition restrict(users: list uid)(P: systemProp): systemProp :=
     fun s =>
-      P (List.filter (fun str => List.existsb (fun a => rel_dec (user (hd str)) a) users) s).
+      P (List.filter (fun str =>
+                        List.existsb (rel_dec (user (hd str))) users) s).
+  Arguments restrict /.
+  
+  Definition noone(P: traceProp): systemProp :=
+    fun s => List.Forall (fun x => ~ (P x)) s.
+  Arguments noone /.
+
+  Definition someone(P: traceProp): systemProp :=
+    fun s => List.Exists P s.
+  Arguments someone /.
   
   Declare Custom Entry etl.
   Declare Scope etl_scope.
 
-  Notation "<{ a '|-' e }>" :=
+  Notation "<{ e }>" := e (at level 0, e custom etl at level 99) : etl_scope.
+  Notation "( x )" := x (in custom etl, x at level 99) : etl_scope.
+  Notation "x" := x (in custom etl at level 0, x constr at level 0) : etl_scope.
+  Notation "'_' '|-' e " :=
+    (noone e)
+      (at level 0, e custom etl at level 99) : etl_scope.
+  Notation "'*' '|-' e " :=
+    (trace2system e)
+      (at level 0, e custom etl at level 99) : etl_scope.
+  Notation "a '|-' e " :=
     (restrict a e)
       (at level 0, a constr, e custom etl at level 99) : etl_scope.
 
-  Notation "( x )" := x (in custom etl, x at level 99) : etl_scope.
-  Notation "x" := x (in custom etl at level 0, x constr at level 0) : etl_scope.
-
-  (********************** Path quantification now *************************)
-  Definition forall_agents(P: traceProp): systemProp :=
-    fun s => List.Forall (fun str => P str) s.
-  
-  Definition exists_agent(P: traceProp): systemProp :=
-    fun s => List.Exists (fun str => P str) s.
-
-  Definition forall_now(P: stateProp): systemProp :=
-    fun s => List.Forall (fun str => P (hd str)) s.
-  
-  Definition exist_now(P: stateProp): systemProp :=
-    fun s => List.Exists (fun str => P (hd str)) s.
-
-  Coercion forall_agents: traceProp >-> systemProp.
-  Coercion system2trace: systemProp >-> traceProp.
-  
   (***************** Property impled by big-step *********************)
   Definition leads_to (P Q : systemProp) : Prop :=
     forall s t , P s -> s ==>* t -> Q t.
 
-  (***************** All the intuitionistic logics! *****************)
-  Global Instance ILogicOps_systemProp : ILogicOps systemProp := _.
+  Notation "a '->*' b" :=
+    (leads_to a b)
+      (in custom etl at level 90, a custom etl, b custom etl,
+        right associativity) : etl_scope.
 
   Notation "x /\ y"   := (land x y) (in custom etl at level 50, left associativity).
   Notation "x \/ y"   := (lor x y) (in custom etl at level 50, left associativity).
-  Notation "'True'"   := (ltrue: systemProp) (in custom etl at level 0).
-  Notation "'False'"  := (lfalse: systemProp) (in custom etl at level 0).
+  Notation "'True'"   := (ltrue) (in custom etl at level 0).
+  Notation "'False'"  := (lfalse) (in custom etl at level 0).
   Notation "x -> y"   := (limpl x y) (in custom etl at level 50, left associativity).
   Notation "x <-> y"   :=
     (land (limpl x y) (limpl y x)) (in custom etl at level 50, left associativity).
@@ -209,7 +236,7 @@ Section ETL.
       P (Continue s str) -> unless P Q str -> unless P Q (Continue s str).
 
   Notation "[] a"  := (always a)  (in custom etl at level 90).
-  Notation "<> a" := (eventually a) (in custom etl at level 90).
+  Notation "{} a" := (eventually a) (in custom etl at level 90).
 
   (****************************** Temporal derived operators ***********************)
   Definition infinitely_often (P : traceProp) : 
@@ -260,7 +287,7 @@ Section ETL.
   Definition rumors(l: list fact): list fact :=    
     List.filter is_rumor l.
 
-  Fixpoint possible_worlds(db: list fact): list (list atom) :=
+  Definition possible_worlds(db: list fact): list (list atom) :=
     List.map (fun l => List.map trust l) (powerset db).
 
   Definition over_db(st: state)(d: list atom): state :=
@@ -270,9 +297,38 @@ Section ETL.
 
   (* For this point in time, knowledge means to consider
      something valid in all possible worlds (Kripke) *)
-  Definition knowledge(P: stateProp): stateProp :=
+  Definition kripke(P: stateProp): stateProp :=
     fun st => forall w, In w (possible_worlds (db st)) ->
                 P st <-> P (over_db st w).
 
+  Definition knows_uid(u: uid)(P: stateProp): systemProp :=
+    fun s => forall a ts, In (Continue a ts) s ->
+          user a = u ->
+          kripke P a.
 
+  Definition knows_all(P: stateProp): systemProp :=
+    fun s => forall a ts, In (Continue a ts) s ->
+                  kripke P a.
+  
+  Notation "'K[' x ']' a" :=
+    (knows_uid x a) (in custom etl at level 90, x constr).
+  Notation "'K[' '*' ']' a" :=
+    (knows_all a) (in custom etl at level 90).
+
+  (********************* Examples ********************)
+  Local Open Scope etl_scope.
+
+  Variable phi: atomProp.
+  Check <{ _ |- {} False }>.
+  Check <{ * |- [] K[*] phi }>.
+  
+  Theorem foo: reflect <{ _ |- {} False }>.
+  Proof.
+    cbv.
+    intros sys HR.
+    induction sys; intros; cbv in *.
+    - constructor.
+    - constructor.
+  Admitted.
+      
 End ETL.
